krivine.v
@@ -20,19 +20,30 @@ Inductive krivine_env : Set :=
   | KEnv: krivine_code -> krivine_env -> krivine_env -> krivine_env
 .
 
-(* State *)
-Inductive krivine_state : Set :=
-  | KState: krivine_code -> krivine_env -> krivine_env -> krivine_state.
+(** a state is (code, env, stack) tuple which may be seen as an environment *)
+Definition krivine_state (c: krivine_code) (e s: krivine_env) : krivine_env :=
+  KEnv c e s
+.
 
-(** 3.3. Semantic: execute one step *)
-Definition krivine_step (st: krivine_state) : option krivine_state :=
+(** Length of an environment list *)
+Fixpoint klength (e: krivine_env) : nat :=
+  match e with
+    | KEnv_nil => O
+    | KEnv _ _ e0 => S (klength e0)
+  end
+.
+
+(** 3.3. Semantic: execute one step.
+  Return KEnv_nil if there were some error, a krivine_state otherwise.
+ *)
+Definition krivine_step (st: krivine_env) : krivine_env :=
   match st with
-    | KState (Access O _) (KEnv c0 e0 _) s => Some (KState c0 e0 s)
-    | KState (Access (S n) c) (KEnv _ _ e) s =>
-        Some (KState (Access n c) e s)
-    | KState (Push c0 c) e s => Some (KState c e (KEnv c0 e s))
-    | KState (Grab c) e (KEnv c0 e0 s) =>
-        Some (KState c (KEnv c0 e0 e) s)
-    | _ => None
+    | KEnv (Access O _) (KEnv c0 e0 _) s => krivine_state c0 e0 s
+    | KEnv (Access (S n) c) (KEnv _ _ e) s =>
+        krivine_state (Access n c) e s
+    | KEnv (Push c0 c) e s => krivine_state c e (KEnv c0 e s)
+    | KEnv (Grab c) e (KEnv c0 e0 s) =>
+        krivine_state c (KEnv c0 e0 e) s
+    | _ => KEnv_nil
   end
 .
